A1:
$$\sqrt{ \vec{b}\cdot \vec{b} } = 3$$
A2:
$$\frac{{\vec{b}\cdot \vec{a}}}{\begin{Vmatrix}
a
\end{Vmatrix}^2}*\vec{a}$$
$$=\frac{5}{5}*\begin{bmatrix}
1 \\
0 \\
2
\end{bmatrix}$$
A3:
$$\begin{vmatrix}
1 & 0 & 2 \\
1 & -2 & 2 \\
1 & 2 & 2
\end{vmatrix}$$
$$= -4+4-(-4+4)$$
$$=0$$
They are linearly dependent
$$\begin{bmatrix}
1 & 1 & 1 & | & 0 \\
0 & -2 & 2 & | & 0 \\
2 & 2 & 2 & | & 0
\end{bmatrix}$$
$$\begin{bmatrix}
1 & 1 & 1 & | & 0 \\
0 & -2 & 2 & | & 0 \\
0 & 0 & 0 & | & 0
\end{bmatrix}$$
$$x_{3}= t$$
$$x_{2} = t$$
$$x_{1} = -2t$$
A4:
$$v_{1} = \begin{bmatrix}
2 \\
0 \\
1
\end{bmatrix}$$
$$v_{2} = \begin{bmatrix}
0 \\
1 \\
1
\end{bmatrix}$$
$$\begin{vmatrix}
\hat{i}&\hat{j}&\hat{k}\\
2 & 0 & 1 \\
0 & 1 & 1
\end{vmatrix}$$
$$= -\hat{i}-2\hat{j}+2\hat{k}$$
$$\begin{bmatrix}
-1 \\
-2 \\
2
\end{bmatrix}$$
$$= \frac{3}{2}$$
A5:
$$x_{2} = 3$$
$$x_{1} = 7-6 = 1$$
A6:
$$x=1+2s$$
$$y = 2+s+3t$$
$$z = 3+t$$
$$t = z-3$$
$$s=\frac{x}{2}-\frac{1}{2}$$
$$y = 2+\frac{x}{2}-\frac{1}{2}+3z-9$$
$$\frac{1}{2}x-y+3z=\frac{15}{2}$$
$$x-2y+6z=15$$
A7:
$$\vec{n} = \begin{bmatrix}
2 \\
4
\end{bmatrix}$$
$$x = 0, y = \frac{1}{2}$$
$$p = \left( 0, \frac{1}{2} \right)$$
$$q = (1,2)$$
$$\vec{v_{qp}} = \begin{bmatrix}
-1 \\
-\frac{3}{2}
\end{bmatrix}$$
$$\vec{u_{n}} = \begin{bmatrix}
1 \\
2
\end{bmatrix}* \frac{1}{\sqrt{ 5 }}$$
$$\vec{v_{qp}}\vec{\cdot}u_{n} = -\frac{1}{\sqrt{ 5 }}-\frac{3}{\sqrt{ 5 }} = -\frac{4}{\sqrt{5  }}$$
A8:
$$\begin{bmatrix}
2 & -2 & | & 0 \\
-1 & 0 & | & -2 \\
0 & -1 & | & -2
\end{bmatrix}$$
$$s = 2, t = 2$$
$$\begin{bmatrix}
5 \\
0 \\
3
\end{bmatrix}$$
A9:
$$d = \begin{bmatrix}
3 \\
1 \\
2
\end{bmatrix}\cdot \begin{bmatrix}
1 \\
3 \\
3
\end{bmatrix} = 12$$
$$v = \begin{bmatrix}
3 \\
2 \\
1
\end{bmatrix}* 3 = \begin{bmatrix}
9 \\
6 \\
3
\end{bmatrix}$$
B1:
$$\begin{bmatrix}
0 & 1 & 2 & | & 2 \\
1 & -1 & 1 & | & -1 \\
4 & -3 & 8 & | & 2
\end{bmatrix}$$
$$ = \begin{bmatrix}
0 & 1 & 2 & | & 2 \\
1 & 0 & 3 & | & 1 \\
4 & -3 & 8 & | & 2
\end{bmatrix}$$
$$ = \begin{bmatrix}
0 & 1 & 2 & | & 2 \\
1 & 0 & 3 & | & 1 \\
0 & -3 & -4 & | & -2
\end{bmatrix}$$
$$=\begin{bmatrix}
0 & 1 & 2 & | & 2 \\
1 & 0 & 3 & | & 1 \\
0 & 0 & 2 & | & 4
\end{bmatrix}$$
$$x_{3} = 2$$
$$x_{1} = -5$$
$$x_{2} = -2$$
$$\begin{bmatrix}
x_{1} \\
x_{2} \\
x_{3}
\end{bmatrix} = \begin{bmatrix}
-5 \\
-2 \\
2
\end{bmatrix}$$
B2:
$$\begin{bmatrix}
1 \\
1 \\
0
\end{bmatrix}\times \begin{bmatrix}
0 \\
3 \\
-1
\end{bmatrix} = \begin{vmatrix}
\hat{i}&\hat{j}&\hat{k}\\
1 & 1 & 0 \\
0 & 3 & -1
\end{vmatrix} = -\hat{i}+\hat{j}+3\hat{k} = t\begin{bmatrix}
-1 \\
1 \\
3
\end{bmatrix} + \vec{p}$$
$$x = 1, y = 1, z = 0$$
$$ L = t\begin{bmatrix}
-1 \\
1 \\
3 
\end{bmatrix} + \begin{bmatrix}
1 \\
1 \\
0 
\end{bmatrix}$$
b.
$$\begin{bmatrix}
2 \\
1 \\
-3
\end{bmatrix}\times \begin{bmatrix}
-1 \\
1 \\
3
\end{bmatrix} = \begin{vmatrix}
\hat{i}&\hat{j}&\hat{k}\\
2 & 1 & -3 \\
-1 & 1 & 3
\end{vmatrix} = 6\hat{i}-3\hat{j}+3\hat{k}$$
$$6x-3y+3z=d$$
$$6x -3y +3z = 3$$
$$2x-y+z=1$$
B3:
$$\begin{bmatrix}
1 & 2 & 2 & | & 0 \\
1 & 2 & 3 & | & k \\
2 & 2+k & 5 & | & k
\end{bmatrix}$$
$$\begin{bmatrix}
1 & 2 & 2 & | & 0 \\
0 & 0 & 1 & | & k \\
2 & 2+k & 5 & | & k
\end{bmatrix}$$
$$\begin{bmatrix}
1 & 2 & 2 & | & 0 \\
0 & 0 & 1 & | & k \\
0 & k-2 & 1 & | & k
\end{bmatrix}$$
$$\begin{bmatrix}
1 & 2 & 2 & | & 0 \\
0 & 0 & 1 & | & k \\
0 & k-2 & 0 & | & 0
\end{bmatrix}$$