See [[Matrix Multiplication]]
$$\begin{cases}
x_{1}+2x_{2}+3x_{3}=1 \\
x_{1}-2x_{2}+3x_{3}=2 \\
2x_{1}+x_{2}-x_{3}=3
\end{cases}$$
$$ = \begin{cases}
\vec{n_{1}}\cdot \vec{x} =1 \\
\vec{n_{2}}\cdot \vec{x} = 2 \\
\vec{n_{3}}\cdot \vec{x} = 3 \\
\end{cases}$$
$$\begin{cases}
\vec{n_{1}} = \begin{bmatrix}
1 & 2 & 3
\end{bmatrix} \\
\vec{n_{2}} = \begin{bmatrix}
1 & -2 & 3 
\end{bmatrix} \\
\vec{n_{3}} = \begin{bmatrix}
2 & 1 & -1
\end{bmatrix}
\end{cases}$$
$$\begin{bmatrix}
\vec{n_{1}} \\
\vec{n_{2}} \\
\vec{n_{3}}
\end{bmatrix} \cdot \vec{x} = \begin{bmatrix}
1 \\
2 \\
3
\end{bmatrix}$$

$$A\vec{x} = \vec{b}$$ 
where $A = \begin{bmatrix}1&2&3\\1&-2&3\\2&1&-1\end{bmatrix}$

