$$\frac{dp}{dt} = kp$$
$$p=Ce^{kt}$$
$$\frac{dp}{dt} = kp(Q-p)$$
$$\int \frac{1}{p(Q-p)} \, dp =kt+C$$
$$\frac{A}{p}+\frac{B}{Q-p}$$
$$A(Q-p)+Bp=1$$
$$p = Q, B=\frac{1}{Q}$$
$$p = 0, A = \frac{1}{Q}$$
$$\int \frac{1}{pQ}+\frac{1}{Q^2-pQ} \, dq $$
$$= \frac{1}{Q}\ln |p|-\frac{1}{Q}\ln|Q-p|$$
$${\frac{{\ln{ \frac{p}{Q-p} }}}{Q}}$$
$$\ln| \frac{p}{Q-p}| = kQt+C$$
$$\frac{p}{Q-p}=Ce^{kQt}$$
$$p +p(kqt)= ekt(Q)$$
$$p(1+Ce^{kQt})=Q*Ce^{kQt}$$
$$p = \frac{QCe^{kQt}}{1+Ce^{kQt}}$$
$$A = \frac{QC}{1+C}$$
$$A+AC=QC$$
$$QC-AC=A$$
$$C(Q-A)=A$$
$$C=\frac{A}{Q-A}$$