a.

| d   | c   | b   | a   | output | num |
| --- | --- | --- | --- | ------ | --- |
| 0   | 0   | 0   | 0   | 1      | 0   |
| 0   | 0   | 0   | 1   | 1      | 1   |
| 0   | 0   | 1   | 0   | 1      | 2   |
| 0   | 0   | 1   | 1   | 1      | 3   |
| 0   | 1   | 0   | 0   | 0      | 4   |
| 0   | 1   | 0   | 1   | 1      | 5   |
| 0   | 1   | 1   | 0   | 0      | 6   |
| 0   | 1   | 1   | 1   | 0      | 7   |
| 1   | 0   | 0   | 0   | 1      | 8   |
| 1   | 0   | 0   | 1   | 0      | 9   |
| 1   | 0   | 1   | 0   | 0      | 10  |
| 1   | 0   | 1   | 1   | 0      | 11  |
| 1   | 1   | 0   | 0   | 0      | 12  |
| 1   | 1   | 0   | 1   | 1      | 13  |
| 1   | 1   | 1   | 0   | 0      | 14  |
| 1   | 1   | 1   | 1   | 0      | 15  |
b.

| dc/ba | 00  | 01  | 11  | 10  |
| ----- | --- | --- | --- | --- |
| 00    | 1   | 1   | 1   | 1   |
| 01    |     | 1   |     |     |
| 11    | x   | x   | x   | x   |
| 10    | 1   |     | x   | x   |
c.
d.
e.
f.
$$\sim d \land \sim c \lor \sim c \land \sim a \land \sim b \lor c \land a \land \sim b$$
$$(\bar{d} \land  \bar{c}) \lor (\bar{c} \land \bar{a} \land \bar{b}) \lor (a \land c \land \bar{b})$$



$$(\bar{d} \land \bar{c}) \lor (d \land \bar{a}) \lor (a \land c \land \bar{b})$$
